theories/diffpriv_simple_pw_again/adequacy_simple.v
@@ -17,103 +17,6 @@ From clutch.diffpriv_simple_pw_again Require Import weakestpre_simple weakestpre
 From clutch.prob Require Import differential_privacy distribution couplings_dp.
 Import uPred.
 
-(* Local Open Scope R.
-
-
-      Definition wp_pre'
-        `{!spec_updateGS (lang_markov prob_lang) Σ, !diffprivWpGS prob_lang Σ, !specG_prob_lang Σ}
-        (* `{!diffprivGS Σ} *)
-          (wp : coPset -d> expr -d> (val -d> iPropO Σ) -d> iPropO Σ) :
-           coPset -d> expr -d> (val -d> iPropO Σ) -d> iPropO Σ := λ E e1 Φ,
-        (match to_val e1 with
-         | Some v => |={E}=> Φ v
-         | None =>
-             ∀ σ1 e1' σ1' ε δ,
-               state_interp σ1 ∗ spec_interp (e1', σ1') ∗ err_interp ε δ ={E,∅}=∗
-               ⌜reducible (e1, σ1)⌝ ∗
-               (* do good things happen if we require S to be reflexive? *)
-               ∃ (S : cfg → cfg → Prop) (ε1 ε2 δ1 δ2 : nonnegreal) (k : nat),
-                 ⌜DPcoupl (prim_step e1 σ1) (pexec k (e1', σ1')) S ε1 δ1⌝ ∗
-                  ⌜ε1 + ε2 <= ε⌝ ∗ ⌜δ1 + δ2 <= δ⌝ ∗
-                  (∀ e2 σ2 e2' σ2',
-
-                      (* (⌜R (e2, σ2) (e2', σ2')⌝ ={∅}=∗
-                          ▷ |={∅,E}=>  (state_interp σ2 ∗ spec_interp (e2', σ2') ∗ err_interp ε2 δ2 ∗ wp E e2 Φ))) *)
-
-
-                      (⌜S (e2, σ2) (e2', σ2')⌝ ={∅}=∗
-                       (▷ (|={∅,⊤}=> state_interp σ2 ∗ spec_interp (e2', σ2') ∗ err_interp ε2 δ2 ∗ wp E e2 Φ))
-                       ∨
-                         (∃ δ2' : val → nonnegreal, (⌜(∀ RES, 0 <= δ2' RES) ∧ ex_seriesC δ2' ∧ nonneg δ2 = SeriesC δ2'⌝ ∗ ▷ |={∅,⊤}=>
-                            ∀ RES : val, state_interp σ2 ∗ spec_interp (e2', σ2') ∗ err_interp ε2 (δ2' RES) ∗
-                            wp E e2 (λ v, ∃ v' : val, ⤇ (of_val v') ∗ ⌜v = RES → v' = RES⌝)))
-                       (* ∨
-                            (▷ |={∅,⊤}=>
-                               state_interp σ2 ∗ spec_interp (e2', σ2') ∗ err_interp ε2 δ2 ∗
-                               ∀ RES : val, WP e2 {{ v, ∃ v' : val, ⤇ (of_val v') ∗ ⌜v = RES → v' = RES⌝ }}) *)
-                      ))
-
-            end)%I.
-
-
-   Local Instance wp_pre_contractive `{!spec_updateGS (lang_markov prob_lang) Σ, !diffprivWpGS prob_lang Σ, !specG_prob_lang Σ} :
-     Contractive wp_pre'.
-   Proof.
-     rewrite /wp_pre' /= => n wp wp' Hwp E e1 Φ.
-     do 40 f_equiv. 2: do 3 f_equiv. all: f_contractive. all: repeat f_equiv ; apply Hwp.
-   Qed.
-
-   Local Definition wp_def' `{!spec_updateGS (lang_markov prob_lang) Σ, !diffprivWpGS prob_lang Σ, !specG_prob_lang Σ} :
-     Wp (iProp Σ) (expr) (val) () :=
-     {| wp := λ _ : (), fixpoint (wp_pre'); wp_default := () |}.
-   Local Definition wp_aux : seal (@wp_def'). Proof. eexists. simpl. Qed.
-   Definition wp' := wp_aux.(unseal).
-   Global Arguments wp' {Λ Σ _}.
-   Global Existing Instance wp'.
-   Local Lemma wp_unseal `{!spec_updateGS (lang_markov Λ) Σ, !diffprivWpGS Λ Σ} : wp =
-     (@wp_def Λ Σ _ _).(wp).
-   Proof. rewrite -wp_aux.(seal_eq) //. Qed.
-
-   Section wp.
-   Context `{!spec_updateGS (lang_markov Λ) Σ, !diffprivWpGS Λ Σ}.
-   Implicit Types P : iProp Σ.
-   Implicit Types Φ : val Λ → iProp Σ.
-   Implicit Types v : val Λ.
-   Implicit Types e : expr Λ.
-   Implicit Types σ : state Λ.
-   Implicit Types ρ : cfg Λ.
-
-   (* Weakest pre *)
-   Lemma wp_unfold E e Φ s :
-     WP e @ s; E {{ Φ }} ⊣⊢ wp_pre (wp (PROP:=iProp Σ) s) E e Φ.
-   Proof. rewrite wp_unseal. apply (fixpoint_unfold wp_pre). Qed.
-
-   Global Instance wp_ne E e n s :
-     Proper (pointwise_relation _ (dist n) ==> dist n) (wp (PROP:=iProp Σ) s E e).
-   Proof.
-     revert e. induction (lt_wf n) as [n _ IH]=> e Φ Ψ HΦ.
-     rewrite !wp_unfold /wp_pre /=.
-     do 39 f_equiv.
-     f_contractive_fin.
-     do 2 f_equiv. rewrite IH ; [done | lia |].
-     intros ?. apply dist_S, HΦ.
-   Qed.
-   Global Instance wp_proper E e s :
-     Proper (pointwise_relation _ (≡) ==> (≡)) (wp (PROP:=iProp Σ) s E e).
-   Proof.
-     by intros Φ Φ' ?; apply equiv_dist=>n; apply wp_ne=>v; apply equiv_dist.
-   Qed.
-   Global Instance wp_contractive E e n s :
-     TCEq (to_val e) None →
-     Proper (pointwise_relation _ (dist_later n) ==> dist n) (wp (PROP:=iProp Σ) s E e).
-   Proof.
-     intros He Φ Ψ HΦ. rewrite !wp_unfold /wp_pre He /=.
-     do 38 f_equiv.
-     f_contractive.
-     repeat f_equiv.
-   Qed. *)
-
-
 Section adequacy.
   Context `{!diffprivGS Σ}.
 
@@ -132,42 +35,6 @@ Section adequacy.
     iApply fupd_mask_intro; [set_solver|]; iIntros "_".
     iPureIntro. by eapply DPcoupl_dret.
   Qed.
-
-  (* Lemma wp_adequacy_step_fupdN n : ∀ ε δ (e e' : expr) (σ σ' : state) φ,
-       state_interp σ ∗ spec_interp (e', σ') ∗ err_interp ε δ ∗
-       WP e {{ v, ∃ v', ⤇ Val v' ∗ ⌜φ v v'⌝ }} ⊢
-       |={⊤,∅}=> |={∅}▷=>^n ⌜DPcoupl (exec n (e, σ)) (lim_exec (e', σ')) φ ε δ⌝.
-     Proof.
-       iInduction n as [|n] "IH" ; iIntros (ε δ e e' σ σ' φ) ;
-         iIntros "(Hσ & HspecI_auth & Hε & Hwp)".
-       { destruct (to_val e) eqn:He.
-         - iMod (wp_adequacy_val_fupd with "[$]") as %?; [done|].
-           by iApply step_fupdN_intro.
-         - iApply fupd_mask_intro; [done|]; iIntros "_ /=".
-           iPureIntro. rewrite He.
-           by apply DPcoupl_dzero.
-       }
-       destruct (language.to_val e) eqn:He.
-       { iMod (wp_adequacy_val_fupd with "[$]") as %?; [done|].
-         iApply step_fupdN_intro; [done|].
-         do 3 iModIntro. done. }
-       iEval (rewrite wp_unfold /wp_pre He) in "Hwp".
-       (* from the assumption Hwp (and the State/Spec/Err interp) we get that... *)
-       (* - there is a R-coupling HCR for the next prim_step and k rhs-steps *)
-       (* - the recursive WP holds later after stepping *)
-       iMod ("Hwp" with "[$]") as "(%red & %R & % & % & % & % & %k & %HCR & %hε & %hδ & Hrec)".
-       (* rewrite the execution in the goal into dbinds *)
-       rewrite exec_Sn /step_or_final ; iSimpl ; rewrite He. rewrite (lim_exec_pexec k).
-       (* bind the coupling HCR *)
-       iApply (step_fupdN_mono _ _ _ ⌜∀ ρ ρ', R ρ ρ' → DPcoupl (exec n ρ) (lim_exec ρ') φ ε2 δ2⌝).
-       { iPureIntro. intros. eapply DPcoupl_dbind'' ; eauto. }
-       rewrite -step_fupdN_Sn. iIntros ([e2 σ2] [e2' σ2'] HR).
-       iSpecialize ("Hrec" $! _ _ _ _ HR).
-       iMod "Hrec". iSimpl ; iIntros "!> !> !>".
-       (* we get the coupling for the remaining n steps from IH with Hrec. *)
-       iMod "Hrec" as "(HT & S & E & Hwp)". iApply ("IH" with "[$]").
-     Qed. *)
-
 
   Lemma wp_adequacy_step_fupdN_pw n : ∀ ε δ (e e' : expr) (σ σ' : state) φ (φrefl : ∀ x, φ x x),
     state_interp σ ∗ spec_interp (e', σ') ∗ err_interp ε δ ∗
@@ -189,50 +56,58 @@ Section adequacy.
       do 3 iModIntro. done. }
     iEval (rewrite wp_unfold) in "Hwp".
 
-    (* eassert ((@wp_pre prob_lang Σ _ _) = (@wp_pre' Σ _ _ _)) as h by admit.
-       iEval (rewrite h /wp_pre') in "Hwp". *)
-
     iEval (rewrite /wp_pre He) in "Hwp".
 
-    (* from the assumption Hwp (and the State/Spec/Err interp) we get that...
-       - there is a R-coupling HCR for the next prim_step and k rhs-steps
-       - the recursive WP holds later after stepping *)
-    iMod ("Hwp" with "[$]") as "(%red & %R & % & % & % & % & %k & %HCR & %hε & %hδ & Hrec)".
-    (* rewrite the execution in the goal into dbinds *)
-    rewrite exec_Sn /step_or_final ; iSimpl ; rewrite He. rewrite (lim_exec_pexec k).
-    (* bind the coupling HCR *)
-    iApply (step_fupdN_mono _ _ _ ⌜∀ ρ ρ', R ρ ρ' → DPcoupl (exec n ρ) (lim_exec ρ') φ ε2 δ2⌝).
-    { iPureIntro. intros. eapply DPcoupl_dbind'' ; eauto. }
-    rewrite -step_fupdN_Sn. iIntros ([e2 σ2] [e2' σ2'] HR).
-    iSpecialize ("Hrec" $! e2 σ2 e2' σ2').
-    assert (∀ x y, eq x y → φ x y) as φpw. { clear -φrefl. intros ?? ->. apply φrefl. }
-
-    set (pweq_res (RES : val) := (λ v v', v = RES → v' = RES)).
-
-
-    (* iAssert (⌜R (e2, σ2) (e2', σ2')⌝ ={∅}=∗
-                (▷ (|={∅,⊤}=> state_interp σ2 ∗ spec_interp (e2', σ2') ∗ err_interp ε2 δ2 ∗ WP e2 {{ v, ∃ v' : val, ⤇ v' ∗ ⌜φ v v'⌝ }}))
-                ∨
-                  (▷ |={∅,⊤}=>
-                     state_interp σ2 ∗ spec_interp (e2', σ2') ∗ err_interp ε2 δ2 ∗
-                     ∀ RES : val, WP e2 {{ v, ∃ v' : val, ⤇ v' ∗ ⌜pweq_res RES v v'⌝ }}))%I with "[-]" as "-#Hrec" ; [admit|]. *)
-
-    iMod ("Hrec" $! HR) as "[Hrec | pw]" ; iSimpl ; iIntros "!>!>!>".
-    - iMod "Hrec" as "(HT & S & E & Hwp)". iApply ("IH" with "[] [$]").
+    iMod ("Hwp" with "[$]") as "[(%red & %R & % & % & % & % & %k & %HCR & %hε & %hδ & Hrec)|pw]".
+    -
+      (* rewrite the execution in the goal into dbinds *)
+      rewrite exec_Sn /step_or_final ; iSimpl ; rewrite He. rewrite (lim_exec_pexec k).
+      (* bind the coupling HCR *)
+      iApply (step_fupdN_mono _ _ _ ⌜∀ ρ ρ', R ρ ρ' → DPcoupl (exec n ρ) (lim_exec ρ') φ ε2 δ2⌝).
+      { iPureIntro. intros. eapply DPcoupl_dbind'' ; eauto. }
+      rewrite -step_fupdN_Sn. iIntros ([e2 σ2] [e2' σ2'] HR).
+      iSpecialize ("Hrec" $! e2 σ2 e2' σ2').
+      iMod ("Hrec" $! HR) as "Hrec" ; iSimpl ; iIntros "!>!>!>".
+      iMod "Hrec" as "(HT & S & E & Hwp)". iApply ("IH" with "[] [$]").
       1: done.
     -
-      iDestruct "pw" as "(%δ2' & (%hpos & %hex & %hδ2) & pw)".
-      iApply (step_fupdN_mono _ _ _ ⌜∀ RES, DPcoupl (exec n (e2, σ2)) (lim_exec (e2', σ2')) (pweq_res RES) ε2 (δ2' RES)⌝).
-      { iPureIntro. rewrite hδ2. intros PWCPL.
+      iDestruct "pw" as "(%e2 & %e2' & %σ2' & %k & %hstep & %hexec & %δ2' & (%hpos & %hex & %hδ) & pw)".
+      assert (∀ x y, eq x y → φ x y) as φpw. { clear -φrefl. intros ?? ->. apply φrefl. }
+
+      set (pweq_res (RES : val) := (λ v v', v = RES → v' = RES)).
+
+      rewrite exec_Sn /step_or_final ; iSimpl ; rewrite He. rewrite (lim_exec_pexec k).
+      iApply (step_fupdN_mono _ _ _ ⌜DPcoupl (exec n (e2, σ)) (lim_exec (e2', σ2')) φ ε δ⌝).
+      { iPureIntro. intros. eapply (DPcoupl_dbind'' 0 ε ε 0 δ) ; try real_solver. 1: apply cond_nonneg.
+        2: apply DPcoupl_pos_R.
+        2: apply DPcoupl_trivial => //.
+        - simpl. intros ρ ρ' (_ & lhs & rhs).
+          assert (ρ = (e2, σ)) as ->.
+          2: assert (ρ' = (e2', σ2')) as -> => //.
+          + admit.
+          + admit.
+        - destruct hstep as [? hstep]. simpl in *.
+          rewrite /prim_step /=.
+          opose proof head_step_mass.
+          admit.
+        - opose proof (dret_mass ((e2', σ2'))) as h. rewrite -h.
+          f_equal. apply pmf_1_eq_dret in hexec. rewrite hexec. done.
+      }
+
+      iApply (step_fupdN_mono _ _ _ ⌜∀ RES, DPcoupl (exec n (e2, σ)) (lim_exec (e2', σ2')) (pweq_res RES) ε (δ2' RES)⌝).
+      { iPureIntro. intros PWCPL.
         eapply DPcoupl_mono ; last first. 4: apply φpw.
         1: eapply DPcoupl_pweq ; last first. 1: eapply PWCPL.
-        all: eauto. 1: apply cond_nonneg. 1,2: right ; reflexivity.
+        all: eauto. 1: apply cond_nonneg. 1: right ; eauto.
       }
+      iIntros "!>!>!>".
       iIntros (RES).
       iMod "pw". iDestruct ("pw" $! RES) as "(HT & S & (ε & δ) & pw)".
-      iApply ("IH" $! ε2 (δ2' RES) e2 e2' σ2 σ2' (pweq_res RES) with "[%] [$]").
-      intros v hv. exact hv.
-  Qed.
+      iApply ("IH" $! ε (δ2' RES) e2 e2' σ σ2' (pweq_res RES) with "[%] [-]").
+      1: intros v hv. 1: exact hv.
+      iFrame.
+
+  Admitted.
 
 
 
