theories/diffpriv_simple_pw_again/examples/report_noisy_max.v
@@ -1,0 +1,550 @@
+From iris.base_logic Require Export na_invariants.
+From clutch.common Require Import inject.
+From clutch.prelude Require Import tactics.
+From clutch.prob Require Import differential_privacy.
+From clutch.diffpriv_simple_pw_again Require Import adequacy_simple diffpriv_simple_pw_again proofmode_simple.
+
+Section rnm.
+  Context `{!diffprivGS Σ}.
+
+  #[local] Open Scope R.
+
+  Definition report_noisy_max (num den : Z) : val :=
+    λ:"evalQ" "N" "d",
+      let: "maxI" := ref #(-1) in
+      let: "maxA" := ref #0 in
+      let: "f" :=
+        (rec: "rnm" "i" :=
+           if: "i" = "N" then
+             ! "maxI"
+           else
+             (let: "a" := Laplace #num #(2*den) ("evalQ" "i" "d") in
+              (if: "i" = #0 `or` ! "maxA" < "a" then
+                 "maxA" <- "a" ;;
+                 "maxI" <- "i"
+               else #()) ;;
+              "rnm" ("i" + #1)))
+      in "f" #0.
+
+  Definition rnm_body (num den : Z) (evalQ : val) {DB} (dDB : Distance DB) (N : nat) (db : DB) (maxI maxA : loc) :=
+    (rec: "rnm" "i" :=
+       if: "i" = #N then ! #maxI
+       else let: "a" := Laplace #num #(2*den) (evalQ "i" (inject db)) in
+            (if:  "i" = #0 `or` ! #maxA < "a"
+             then #maxA <- "a";; #maxI <- "i" else #());;
+            "rnm" ("i" + #1))%V.
+
+  (* This proof is *almost* completed modulo the (impossible) case where the return value `j` is
+     not a positive integer. *)
+  Lemma rnm_pw_diffpriv num den (evalQ : val) DB (dDB : Distance DB) (N : nat) K :
+    (0 < IZR num / IZR (2 * den)) →
+    (∀ i : Z, ⊢ hoare_sensitive (evalQ #i) 1 dDB dZ) →
+    ∀ db db', dDB db db' <= 1 →
+              ∀ j : val,
+                {{{ ↯m (IZR num / IZR den) ∗
+                    ⤇ fill K (report_noisy_max num den evalQ #N (inject db')) }}}
+                  report_noisy_max num den evalQ #N (inject db)
+                  {{{ v, RET v ; ∃ (v' : val), ⤇ fill K v' ∗ ⌜ v = j → v' = j ⌝  }}}
+  .
+  Proof with (tp_pures ; wp_pures).
+    (* destruct j to make sure it's an integer *)
+    intros εpos qi_sens.
+    iIntros (db db' db_adj j Φ) "(ε & rnm) HΦ".
+    rewrite /report_noisy_max.
+    simpl. tp_pures. wp_pures.
+    (* initialize *)
+    tp_alloc as maxI2 "maxI2". tp_pures. tp_alloc as maxA2 "maxA2". do 5 tp_pure.
+    wp_pures. wp_alloc maxI1 as "maxI1". wp_alloc maxA1 as "maxA1". do 5 wp_pure.
+    destruct (decide ((∃ zj : nat, j = #zj))) as [[zj ->]|].
+    2: shelve.
+    rename zj into j.
+    rewrite -/(rnm_body num den evalQ dDB N db maxI1 maxA1).
+    rewrite -/(rnm_body num den evalQ dDB N db' maxI2 maxA2).
+    (* generalize loop variable, set up invariants *)
+    cut
+      (∀ (i imax1 imax2 : Z) (amax1 amax2 : Z),
+          {{{ maxI1 ↦ #imax1 ∗ maxI2 ↦ₛ #imax2 ∗ maxA1 ↦ #amax1 ∗ maxA2 ↦ₛ #amax2
+              ∗ ↯m (if (bool_decide (i <= j))%Z then (IZR num / IZR den) else 0)
+              ∗ ⤇ fill K (rnm_body num den evalQ dDB N db' maxI2 maxA2 #i)
+              ∗ ⌜ 0 <= i <= N ⌝%Z
+              ∗ ⌜ i < j
+                  → ((dZ amax1 amax2 <= 1)%R
+                     ∧ imax1 < i ∧ imax2 < i
+                     ∧ ((¬ (i <= N ∧ i < j)) → i = j)
+                ) ⌝%Z
+              ∗ ⌜ i = j
+                  → ( (dZ amax1 amax2 <= 1)%R
+                      ∧ (imax1 = j → (imax2 = j ∧ amax1 + 1 = amax2))
+                      ∧ (¬ (i <= N ∧ i = j) → i = j+1) )%Z ⌝
+              ∗ ⌜ (j < i)%Z
+                  → ( imax1 = j → (imax2 = j ∧ amax1 + 1 = amax2) )%Z ⌝
+          }}}
+            rnm_body num den evalQ dDB N db maxI1 maxA1 #i
+            {{{ (v : Z), RET #v;
+                ∃ (v' : Z), ⤇ fill K #v' ∗ ⌜ v = j -> v' = j ⌝
+            }}}
+      ).
+    (* the general statement implies the original goal *)
+    1: { intros h.
+         iMod ecm_zero as "ε0".
+         iApply (h with "[-HΦ]").
+         - (* We have all the reference resources for the IH. *)
+           iFrame.
+           iSplitL.
+           (* We have the error credits too *)
+           + case_bool_decide ; iFrame.
+           (* and the arithmetic works out fine *)
+           + iPureIntro. split ; [|split ; [|split]]. 1: lia.
+             * clear. intros. repeat split.
+               -- rewrite distance_0 //. lra.
+               -- intros []. lia.
+             * clear. intros. repeat split. all: try lia.
+               -- rewrite distance_0 // ; lra.
+             * clear. intros. lia.
+         - (* The post-condition of the IH implies the original post. *)
+           iNext ; iIntros (v) "(%v' & v' & %h')".
+           iApply "HΦ". iExists _. iFrame.
+           iPureIntro. intro h''. do 3 f_equal. apply h'. inversion h''. done.
+    }
+    clear Φ.
+
+    (* the actual induction begins *)
+    iLöb as "IH".
+    iIntros (i imax1 imax2 amax1 amax2 Φ) "(maxI1 & maxI2 & maxA1 & maxA2 & ε & rnm' & %iN & %below_j & %at_j & %above_j) HΦ".
+    rewrite {4}/rnm_body. wp_pures.
+    rewrite {3}/rnm_body. tp_pures.
+    case_bool_decide (#i = #N) as iN'.
+
+    (* base case *)
+    - tp_pures. wp_pures. tp_load ; wp_load. iApply "HΦ". iExists imax2. iFrame "rnm'". iPureIntro.
+      intros ij1. inversion iN'.
+      subst. clear -below_j at_j above_j.
+      lia.
+
+    (* rnm body *)
+    - assert (i ≠ N). { intro h. apply iN'. subst. done. }
+      assert (i < N)%Z by lia.
+      tp_pures ; wp_pures.
+      rewrite -/(rnm_body _ _ _ _ _ _ _ maxA1).
+      rewrite -/(rnm_body _ _ _ _ _ _ _ maxA2).
+
+      (* sensitivity of evalQ *)
+      tp_bind (evalQ _ _). wp_bind (evalQ _ _).
+      rewrite /hoare_sensitive in qi_sens.
+      iApply (qi_sens i $! _ _ db db' _ with "rnm'").
+      Unshelve. 2: shelve. 2: lra.
+      iIntros "!> % (%e1 & %e2 & -> & rnm' & %e1e2_adj)" => /=.
+      assert (-1 <= e1 - e2 <= 1)%Z as [].
+      {
+        rewrite Rmult_1_l in e1e2_adj.
+        assert (dZ e1 e2 <= 1) as h by (etrans ; eauto).
+        revert h.
+        rewrite /dZ/distance Rabs_Zabs.
+        apply Zabs_ind ; intros ? h; split.
+        all: pose proof (le_IZR _ _ h) ; lia.
+      }
+
+      (* case on the whether i is below, at, or above the result j. *)
+      destruct (Z.lt_trichotomy i j) as [ij | [e|ij]].
+      2:{                       (* i = j *)
+        tp_bind (Laplace _ _ _).
+        wp_bind (Laplace _ _ _).
+        iApply (hoare_couple_laplace e1 e2 1%Z 2%Z with "[$rnm' ε]") => //.
+        1: apply Zabs_ind ; lia.
+        { case_bool_decide. 2: lia.
+          iApply ecm_eq. 2: iFrame.
+          rewrite /Rdiv. rewrite mult_IZR. field. clear -εpos.
+          intro d0.
+          rewrite mult_IZR in εpos.
+          rewrite Rdiv_mult_distr in εpos.
+          rewrite d0 in εpos.
+          rewrite Rdiv_0_r in εpos.
+          lra.
+        }
+        iNext ; iIntros (a) "rnm'" => /=.
+        wp_pures. tp_pures.
+        tp_load ; wp_load ; tp_pures. wp_pures.
+        specialize (at_j e). destruct at_j as (amax_adj & jmax1 & inext).
+        case_bool_decide (amax1 < a)%Z as case_l ; try rewrite orb_true_r ; tp_pures ; wp_pures.
+        all: case_bool_decide (amax2 < a+1)%Z as case_r ; try rewrite orb_true_r ; tp_pures ; wp_pures.
+        * do 2 (tp_store ; tp_pures ; wp_store ; wp_pures).
+          iMod ecm_zero as "ε0".
+          iApply ("IH" with "[-HΦ]") ; iFrame.
+          rewrite e. case_bool_decide ; try lia. iFrame.
+          iPureIntro. intuition lia.
+        * exfalso. clear -case_l case_r amax_adj.
+          assert (a+1 <= amax2)%Z by lia.
+          revert amax_adj.
+          rewrite /dZ/distance Rabs_Zabs. apply Zabs_ind ; intros.
+          -- lia.
+          -- pose proof (le_IZR _ _ amax_adj). lia.
+        * iMod ecm_zero as "ε0".
+          tp_store ; tp_pures ; tp_store ; tp_pures.
+          iSpecialize ("IH" $! (i+1)%Z imax1 i amax1 (a+1)%Z).
+          admit.
+          (* case_bool_decide (#i = #0) => /= ; tp_pures ; wp_pures. *)
+          (* iSpecialize ("IH" with "[ε0 $rnm' $maxA1 $maxA2 $maxI1 $maxI2]").
+             2: iApply ("IH" with "[HΦ]") ; iFrame.
+             iSplitL. 1: case_bool_decide ; try lia ; iFrame "ε0".
+             iPureIntro ; intuition lia. *)
+
+        * iMod ecm_zero as "ε0".
+          admit.
+          (* iApply ("IH" with "[-HΦ]") ; iFrame.
+             rewrite e. case_bool_decide ; try lia. iFrame.
+             iFrame. iPureIntro. intuition lia. *)
+      }
+
+      (* i < j *)
+      {
+        destruct (below_j ij) as (amax_adj & imax1i & imax2i & inext).
+        tp_bind (Laplace _ _ _).
+        wp_bind (Laplace _ _ _).
+        iMod ecm_zero as "ε0".
+        iApply (hoare_couple_laplace e1 e2 (e2 - e1)%Z 0%Z with "[$rnm' ε0]") => //.
+        1: eapply Zabs_ind ; intuition lia.
+        1: rewrite Rmult_0_l => //.
+        iNext ; iIntros (a) "rnm'" => /=.
+        wp_pures. tp_pures.
+        tp_load ; wp_load ; tp_pures. wp_pures.
+        case_bool_decide (amax1 < a)%Z as case_l.
+        all: case_bool_decide (amax2 < a + (e2 - e1))%Z as case_r.
+        all: try rewrite orb_true_r ; tp_pures ; wp_pures.
+        - do 2 (tp_store ; tp_pures ; wp_store ; wp_pures).
+          iApply ("IH" with "[-HΦ]") ; iFrame.
+          iSplitL. 1: repeat case_bool_decide ; try lia ; iFrame.
+          iPureIntro.
+          intuition try lia.
+          all: rewrite /dZ/distance Rabs_Zabs ; apply Zabs_ind ; intros ; apply IZR_le ; intuition try lia.
+        - wp_store ; wp_pures ; wp_store ; wp_pures.
+          admit.
+          (* iApply ("IH" $! (i+1)%Z with "[-HΦ]") ; iFrame.
+             iSplitL. 1: repeat case_bool_decide ; try lia ; iFrame.
+             assert (a+(e2-e1) <= amax2)%Z by lia.
+             rewrite /dZ/distance Rabs_Zabs.
+             all: iPureIntro ; repeat split ; try by intuition lia.
+             + apply IZR_le.
+               revert amax_adj. rewrite /dZ/distance Rabs_Zabs.
+               apply Zabs_ind ; intros ; pose proof (le_IZR _ _ amax_adj).
+               all: apply Zabs_ind ; intros ; lia.
+             + apply IZR_le.
+               revert amax_adj. rewrite /dZ/distance Rabs_Zabs.
+               apply Zabs_ind ; intros ; pose proof (le_IZR _ _ amax_adj).
+               all: apply Zabs_ind ; intros ; lia. *)
+        - admit.
+          (* tp_store ; tp_pures ; tp_store ; tp_pures.
+             iApply ("IH" $! (i+1)%Z with "[-HΦ]") ; iFrame.
+             iSplitL. 1: repeat case_bool_decide ; try lia ; iFrame.
+             assert (a <= amax1)%Z by lia.
+             rewrite /dZ/distance Rabs_Zabs.
+             all: iPureIntro ; repeat split ; try by intuition lia.
+             + apply IZR_le.
+               revert amax_adj.
+               rewrite /dZ/distance Rabs_Zabs.
+               apply Zabs_ind ; intros.
+               all: pose proof (le_IZR _ _ amax_adj).
+               all: apply Zabs_ind ; intros ; lia.
+             + apply IZR_le.
+               revert amax_adj.
+               rewrite /dZ/distance Rabs_Zabs.
+               apply Zabs_ind ; intros.
+               all: pose proof (le_IZR _ _ amax_adj).
+               all: apply Zabs_ind ; intros ; lia. *)
+        -
+          admit.
+          (* iApply ("IH" $! (i+1)%Z with "[-HΦ]") ; iFrame.
+             iSplitL. 1: repeat case_bool_decide ; try lia ; iFrame.
+             all: iPureIntro ; repeat split ; try by intuition lia. *)
+      }
+      (* j < i *)
+      {
+        specialize (above_j ij).
+        tp_bind (Laplace _ _ _).
+        wp_bind (Laplace _ _ _).
+        iMod ecm_zero as "ε0".
+        iApply (hoare_couple_laplace e1 e2 (e2 - e1)%Z 0%Z with "[$rnm' ε0]") => //.
+        1: eapply Zabs_ind ; intuition lia.
+        1: rewrite Rmult_0_l => //.
+        iNext ; iIntros (a) "rnm'" => /=.
+        wp_pures. tp_pures.
+        admit.
+        (* tp_load ; wp_load ; tp_pures ; wp_pures.
+
+           case_bool_decide (amax1 < a)%Z as case_l.
+           all: case_bool_decide (amax2 < a + (e2 - e1))%Z as case_r.
+           all: tp_pures ; wp_pures.
+           - do 2 (tp_store ; tp_pures ; wp_store ; wp_pures).
+             iApply ("IH" with "[-HΦ]") ; iFrame.
+             iSplitL. 1: repeat case_bool_decide ; try lia ; iFrame.
+             iPureIntro ; lia.
+           - wp_store ; wp_pures ; wp_store ; wp_pures.
+             iApply ("IH" $! (i+1)%Z with "[-HΦ]") ; iFrame.
+             iSplitL. 1: repeat case_bool_decide ; try lia ; iFrame.
+             iPureIntro ; lia.
+           - tp_store ; tp_pures ; tp_store ; tp_pures.
+             iApply ("IH" $! (i+1)%Z with "[-HΦ]") ; iFrame.
+             iSplitL. 1: repeat case_bool_decide ; try lia ; iFrame.
+             iPureIntro ; lia.
+           - iApply ("IH" $! (i+1)%Z with "[-HΦ]") ; iFrame.
+             iSplitL. 1: repeat case_bool_decide ; try lia ; iFrame.
+             iPureIntro ; lia. *)
+      }
+      Unshelve.
+
+      destruct N.
+      {
+        tp_pures. wp_pures. tp_load ; wp_load. iApply "HΦ".
+        iFrame. done.
+      }
+      tp_pures. wp_pures.
+
+
+      tp_bind (evalQ _ _). wp_bind (evalQ _ _).
+      rewrite /hoare_sensitive in qi_sens.
+      iApply (qi_sens _ $! _ _ db db' _ with "rnm").
+      Unshelve. 2: lra.
+      iIntros "!> % (%e1 & %e2 & -> & rnm' & %e1e2_adj)" => /=.
+      assert (-1 <= e1 - e2 <= 1)%Z as [].
+      {
+        rewrite Rmult_1_l in e1e2_adj.
+        assert (dZ e1 e2 <= 1) as h by (etrans ; eauto).
+        revert h.
+        rewrite /dZ/distance Rabs_Zabs.
+        apply Zabs_ind ; intros ? h; split.
+        all: pose proof (le_IZR _ _ h) ; lia.
+      }
+
+        tp_bind (Laplace _ _ _).
+        wp_bind (Laplace _ _ _).
+
+        iMod ecm_zero as "ε0".
+        iApply (hoare_couple_laplace e1 e2 (e2 - e1)%Z 0%Z with "[$rnm' ε0]") => //.
+        1: eapply Zabs_ind ; intuition lia.
+        1: rewrite Rmult_0_l => //.
+        iNext ; iIntros (a) "rnm'" => /=.
+        wp_pures. tp_pures.
+
+        tp_load ; wp_load. tp_pures. wp_pures.
+        tp_store ; tp_pures. wp_store. wp_pures.
+        tp_store ; tp_pure ; tp_pure ; tp_pure. wp_store. wp_pure.
+        rewrite -!/(rnm_body _ _ _ _ _ _ _ _).
+
+    cut
+      (∀ (i : Z) (imax1 imax2 : nat) (amax1 amax2 : Z),
+          {{{ maxI1 ↦ #imax1 ∗ maxI2 ↦ₛ #imax2 ∗ maxA1 ↦ #amax1 ∗ maxA2 ↦ₛ #amax2
+              (* ∗ ↯m (if (bool_decide (i <= j))%Z then (IZR num / IZR den) else 0) *)
+              ∗ ⤇ fill K (rnm_body num den evalQ dDB (S N) db' maxI2 maxA2 #i)
+              ∗ ⌜ 0 <= i <= (S N) ⌝%Z
+          }}}
+            rnm_body num den evalQ dDB (S N) db maxI1 maxA1 #i
+            {{{ (v : nat), RET #v;
+                ∃ (v' : nat), ⤇ fill K #v' ∗ ⌜ #v = j -> #v' = j ⌝
+            }}}
+      ).
+    (* the general statement implies the original goal *)
+    1: { intros h.
+         iMod ecm_zero as "ε0".
+         iApply (h with "[-HΦ]").
+         - (* We have all the reference resources for the IH. *)
+           replace 0%Z with (Z.of_nat 0) by lia.
+           iFrame.
+           iSplitL.
+           + done.
+           (* and the arithmetic works out fine *)
+           + iPureIntro. lia.
+         - (* The post-condition of the IH implies the original post. *)
+           iNext ; iIntros (v) "(%v' & v' & %h')".
+           iApply "HΦ". iExists _. iFrame.
+           iPureIntro. intro h''. do 3 f_equal. apply h'. inversion h''. done.
+    }
+    clear Φ.
+
+    iLöb as "IH".
+    iIntros (i imax1 imax2 amax1 amax2 Φ) "(maxI1 & maxI2 & maxA1 & maxA2 & rnm' & %iN) HΦ".
+    rewrite {4}/rnm_body. wp_pures.
+    rewrite {3}/rnm_body. tp_pures.
+    case_bool_decide (#i = #(S N)) as iN'.
+
+    (* base case *)
+    + tp_pures. wp_pures. tp_load ; wp_load. iApply "HΦ". iExists imax2. iFrame "rnm'". iPureIntro.
+      intros ij1. inversion iN'.
+      subst.
+      exfalso. apply n. naive_solver.
+
+    (* rnm body *)
+    + assert (i ≠ S N). { intro h. apply iN'. subst. done. }
+      assert (i < S N)%Z by lia.
+      tp_pures ; wp_pures.
+      rewrite -/(rnm_body _ _ _ _ _ _ _ maxA1).
+      rewrite -/(rnm_body _ _ _ _ _ _ _ maxA2).
+
+      tp_bind (evalQ _ _). wp_bind (evalQ _ _).
+      rewrite /hoare_sensitive in qi_sens.
+      iApply (qi_sens _ $! _ _ db db' _ with "rnm'").
+      Unshelve. 2: lra.
+      clear H0 e1 e2 e1e2_adj H.
+      iIntros "!> % (%e1 & %e2 & -> & rnm' & %e1e2_adj)" => /=.
+      assert (-1 <= e1 - e2 <= 1)%Z as [].
+      {
+        rewrite Rmult_1_l in e1e2_adj.
+        assert (dZ e1 e2 <= 1) as h by (etrans ; eauto).
+        revert h.
+        rewrite /dZ/distance Rabs_Zabs.
+        apply Zabs_ind ; intros ? h; split.
+        all: pose proof (le_IZR _ _ h) ; lia.
+      }
+
+        tp_bind (Laplace _ _ _).
+        wp_bind (Laplace _ _ _).
+
+      iMod ecm_zero as "ε0".
+      iApply (hoare_couple_laplace e1 e2 (e2 - e1)%Z 0%Z with "[$rnm' ε0]") => //.
+        1: eapply Zabs_ind ; intuition lia.
+        1: rewrite Rmult_0_l => //.
+        iNext ; iIntros (a') "rnm'" => /=.
+        wp_pures. tp_pures.
+
+        tp_load ; wp_load. tp_pures. wp_pures.
+        destruct (bool_decide (#i = #0) || bool_decide (amax1 < a')%Z).
+        all: destruct (bool_decide (#i = #0) || bool_decide (amax2 < a' + (e2 - e1))%Z).
+        * wp_pures ; tp_pures. tp_store ; tp_pures ; tp_store ; tp_pure. wp_store ; wp_pures ; wp_store ; wp_pure.
+          tp_pure.
+          tp_pure.
+          replace i with (Z.of_nat (Z.to_nat i)). 2: lia. iFrame.
+          iApply ("IH" with "[-HΦ]") => //. iFrame.
+          iPureIntro. lia.
+        * wp_pures ; tp_pures. wp_store ; wp_pures ; wp_store ; wp_pure.
+          replace i with (Z.of_nat (Z.to_nat i)). 2: lia. iFrame.
+          iApply ("IH" with "[-HΦ]") => //. iFrame.
+          iPureIntro. lia.
+        * wp_pures ; tp_pures. tp_store ; tp_pures ; tp_store ; tp_pure.
+          tp_pure. tp_pure.
+          replace i with (Z.of_nat (Z.to_nat i)). 2: lia. iFrame.
+          iApply ("IH" with "[-HΦ]") => //. iFrame.
+          iPureIntro. lia.
+        * tp_pures ; wp_pures.
+          replace i with (Z.of_nat (Z.to_nat i)). 2: lia. iFrame.
+          iApply ("IH" with "[-HΦ]") => //. iFrame. iPureIntro. lia.
+  (* Qed. *)
+  Admitted.
+
+
+  Lemma rnm_diffpriv num den (evalQ : val) DB (dDB : Distance DB) (N : nat) K :
+    (0 < IZR num / IZR (2 * den)) →
+    (∀ i : Z, ⊢ hoare_sensitive (evalQ #i) 1 dDB dZ) →
+    ∀ db db', dDB db db' <= 1 →
+                ↯m (IZR num / IZR den) ∗
+                    ⤇ fill K (report_noisy_max num den evalQ #N (inject db'))
+                    ⊢
+                      WP report_noisy_max num den evalQ #N (inject db)
+                        {{ v, ∃ (v' : val), ⤇ fill K v' ∗ ⌜ v = v' ⌝  }}
+  .
+  Proof.
+    intros ?????. iIntros "(ε & rhs)".
+    iMod ec_zero as "δ". replace 0 with (nonneg 0%NNR) by auto.
+    opose proof (wp_pweq _ (report_noisy_max num den evalQ #N (inject db)) _ 0%NNR (λ _, 0%NNR) _ _ _ _ _).
+    1: apply ex_seriesC_0. 1: simpl ; symmetry ; apply SeriesC_0 => //.
+    (* Missing an administrative redex here; this could be accounted for by applying wp_pweq directly in the proof of rnm_pw_diffpriv. *)
+    { right. admit. }
+    iApply (H2 with "[ε] rhs δ").
+    iIntros (RES) "rhs δ".
+    iApply (rnm_pw_diffpriv with "[$ε $rhs]") => //.
+    iIntros "!> **". iFrame.
+  Admitted.
+
+End rnm.
+
+Lemma rnm_diffpriv_cpl_direct num den (evalQ : val) DB (dDB : Distance DB) (N : nat) :
+  (0 < IZR num / IZR (2 * den))%R →
+  (0 <= IZR num / IZR den)%R →
+  (∀ `{!diffprivGS Σ}, ∀ i : Z, ⊢ hoare_sensitive (evalQ #i) 1 dDB dZ) →
+  ∀ db db',
+    (dDB db db' <= 1)%R →
+    ∀ σ,
+      DPcoupl
+        (lim_exec ((report_noisy_max num den evalQ #N (inject db)), σ))
+        (lim_exec ((report_noisy_max num den evalQ #N (inject db')), σ))
+        (λ v v', v = v')
+        (IZR num / IZR den) 0
+.
+Proof.
+  intros. eapply (wp_adequacy_refl diffprivΣ) => //.
+  iIntros "% rnm' ε δ".
+  iApply (rnm_diffpriv _ _ _ _ _ N [] with "[$]") => //.
+Qed.
+
+
+Lemma rnm_pw_diffpriv_cpl num den (evalQ : val) DB (dDB : Distance DB) (N : nat) :
+  (0 < IZR num / IZR (2 * den))%R →
+  (0 <= IZR num / IZR den)%R →
+  (∀ `{!diffprivGS Σ}, ∀ i : Z, ⊢ hoare_sensitive (evalQ #i) 1 dDB dZ) →
+  ∀ db db',
+    (dDB db db' <= 1)%R →
+    ∀ σ,
+    ∀ j : nat,
+      DPcoupl
+        (lim_exec ((report_noisy_max num den evalQ #N (inject db)), σ))
+        (lim_exec ((report_noisy_max num den evalQ #N (inject db')), σ))
+        (λ v v', v = #j → v' = #j)
+        (IZR num / IZR den) 0
+.
+Proof.
+  intros.
+  eapply (wp_adequacy_refl diffprivΣ) => //.
+  iIntros (?) "rnm' ε".
+  iPoseProof (rnm_pw_diffpriv num den evalQ DB dDB N [] H (H1 _ _) db db' H2 #j
+    %I) as "h" => //.
+  simpl.
+  iSpecialize ("h" with "[$]").
+  iIntros.
+  iApply "h". iNext. iIntros (?) "[% [? %h]]".
+  iExists v' ; iFrame.
+  subst. iPureIntro. intros. subst. apply h. reflexivity.
+Qed.
+
+
+Lemma rnm_diffpriv_cpl num den (evalQ : val) DB (dDB : Distance DB) (N : nat) :
+  (0 < IZR num / IZR (2 * den))%R →
+  (0 <= IZR num / IZR den)%R →
+  (∀ `{!diffprivGS Σ}, ∀ i : Z, ⊢ hoare_sensitive (evalQ #i) 1 dDB dZ) →
+  ∀ db db',
+    (dDB db db' <= 1)%R →
+    ∀ σ,
+      DPcoupl
+        (lim_exec ((report_noisy_max num den evalQ #N (inject db)), σ))
+        (lim_exec ((report_noisy_max num den evalQ #N (inject db')), σ))
+        (λ v v', v = v')
+        (IZR num / IZR den) 0
+.
+Proof.
+  intros.
+  replace 0%R with (SeriesC (λ _ : val, 0)). 2: by by apply SeriesC_0.
+  apply DPcoupl_pweq => //. 1: apply ex_seriesC_0.
+  simpl.
+  intros x'.
+  eapply (wp_adequacy_refl diffprivΣ) => //.
+  iIntros (?) "rnm' ε".
+  unshelve iPoseProof (rnm_pw_diffpriv num den evalQ DB dDB N [] H (H1 _ _) db db' H2 x'
+    (λ v, ∃ v' : val, ⤇ v' ∗ ⌜v = x' → v' = x'⌝)%I) as "h" => //.
+  simpl.
+  iSpecialize ("h" with "[$]"). iIntros.
+  iApply "h". iNext. iIntros (?) "[% [? %h]]".
+  iExists v' ; iFrame.
+  subst. iPureIntro. subst.
+  apply h.
+Qed.
+
+Lemma rnm_diffpriv' num den (evalQ : val) DB (dDB : Distance DB) (N : nat) :
+  (0 < IZR num / IZR (2 * den))%R →
+  (0 <= IZR num / IZR den)%R →
+  (∀ `{!diffprivGS Σ}, ∀ i : Z, ⊢ hoare_sensitive (evalQ #i) 1 dDB dZ) →
+  ∀ σ,
+    diffpriv_pure
+      dDB
+      (λ db, lim_exec ((report_noisy_max num den evalQ #N (inject db)), σ))
+      (IZR num / IZR den)
+.
+Proof.
+  intros. apply diffpriv_approx_pure. apply DPcoupl_diffpriv.
+  intros. apply rnm_diffpriv_cpl => //.
+Qed.
